a bit more structure

dev2015/fsub0.v
@@ -39,14 +39,14 @@ Inductive tm : Type :=
   | tapp : tm -> tm -> tm (* f(x) *)
   | tabs : tm -> tm (* \f x.y *)
   | ttapp : tm -> ty -> tm (* f[X] *)
-  | ttabs : tm -> tm (* \f x.y *)
+  | ttabs : ty -> tm -> tm (* \f x.y *)
 .
 
 Inductive vl : Type :=
-| vty   : ty -> vl
+| vty   : list vl -> ty -> vl
 | vbool : bool -> vl
 | vabs  : list vl -> tm -> vl
-| vtabs : list vl -> tm -> vl
+| vtabs : list vl -> ty -> tm -> vl
 .
 
 Definition venv := list vl.
@@ -167,7 +167,11 @@ Hint Unfold closed.
 
 Inductive stp: tenv -> ty -> ty -> Prop :=
 | stp_refl: forall G1 T,
-   stp G1 T T.
+    stp G1 T T
+| stp_sel1: forall G1 T x,
+    index x G1 = Some (TMem T) ->
+    stp G1 (TSel x) T
+.
 (* TODO *)
 
 Inductive has_type : tenv -> tm -> ty -> Prop :=
@@ -200,9 +204,23 @@ Does it make a difference? It seems like we can always widen f?
 *)                    
 | t_tabs: forall env y T1 T2,
            (forall G2, sub_env env G2 -> has_type ((TMem T1)::G2) y (open (TSel (length G2)) T2)) -> 
-           has_type env (ttabs y) (TAll T1 T2)
+           has_type env (ttabs T1 y) (TAll T1 T2)
 (* TODO: sumsumption *)
 .
+
+
+Inductive stp2: venv -> ty -> venv -> ty -> Prop :=
+| stp2_refl: forall G1 G2 T,
+   stp2 G1 T G2 T
+| stp2_sel1: forall G1 G2 GX TX x T2,
+   index x G1 = Some (vty GX TX) ->
+   stp2 GX TX G2 T2 ->
+   stp2 G1 (TSel x) G2 T2
+.
+
+
+
+
 
 Inductive wf_env : venv -> tenv -> Prop := 
 | wfe_nil : wf_env nil nil
@@ -212,18 +230,23 @@ Inductive wf_env : venv -> tenv -> Prop :=
     wf_env (cons v vs) (cons t ts)
 
 with val_type : venv -> vl -> ty -> Prop :=
-| v_ty: forall venv T1,
-    val_type venv vty (TMem T1)
-| v_bool: forall venv b,
-    val_type venv (vbool b) TBool
-| v_abs: forall env venv tenv y T1 T2,
+| v_ty: forall env venv tenv T1 TE,
+    wf_env venv tenv -> (* T1 wf in tenv ? *)
+    stp2 venv (TMem T1) env TE ->
+    val_type env (vty venv T1) TE
+| v_bool: forall venv b TE,
+    stp2 [] TBool venv TE ->
+    val_type venv (vbool b) TE
+| v_abs: forall env venv tenv y T1 T2 TE,
     wf_env venv tenv ->
     has_type (T1::(TFun T1 T2)::tenv) y T2 ->
-    val_type env (vabs venv y) (TFun T1 T2)
-| v_tabs: forall env venv tenv y T1 T2,
+    stp2 venv (TFun T1 T2) env TE -> 
+    val_type env (vabs venv y) TE
+| v_tabs: forall env venv tenv y T1 T2 TE,
     wf_env venv tenv ->
     (forall G2, sub_env tenv G2 -> has_type ((TMem T1)::G2) y (open (TSel (length G2)) T2)) ->
-    val_type env (vtabs venv y) (TAll T1 T2)
+    stp2 venv (TAll T1 T2) env TE ->
+    val_type env (vtabs venv T1 y) TE
 .
 
 
@@ -246,7 +269,7 @@ Fixpoint teval(n: nat)(env: venv)(t: tm){struct n}: option (option vl) :=
         | tfalse     => Some (Some (vbool false))
         | tvar x     => Some (index x env)
         | tabs y     => Some (Some (vabs env y))
-        | ttabs y    => Some (Some (vtabs env y))
+        | ttabs T y  => Some (Some (vtabs env T y))
         | tapp ef ex   =>
           match teval n env ex with
             | None => None
@@ -256,8 +279,8 @@ Fixpoint teval(n: nat)(env: venv)(t: tm){struct n}: option (option vl) :=
                 | None => None
                 | Some None => Some None
                 | Some (Some (vbool _)) => Some None
-                | Some (Some (vty)) => Some None
-                | Some (Some (vtabs _ _)) => Some None
+                | Some (Some (vty _ _)) => Some None
+                | Some (Some (vtabs _ _ _)) => Some None
                 | Some (Some (vabs env2 ey)) =>
                   teval n (vx::(vabs env2 ey)::env2) ey
               end
@@ -267,10 +290,10 @@ Fixpoint teval(n: nat)(env: venv)(t: tm){struct n}: option (option vl) :=
             | None => None
             | Some None => Some None
             | Some (Some (vbool _)) => Some None
-            | Some (Some (vty)) => Some None
+            | Some (Some (vty _ _)) => Some None
             | Some (Some (vabs _ _)) => Some None
-            | Some (Some (vtabs env2 ey)) =>
-              teval n (vty::env2) ey
+            | Some (Some (vtabs env2 T ey)) =>
+              teval n ((vty env2 T)::env2) ey
           end
       end
   end.
@@ -326,16 +349,8 @@ Proof.
 Qed.
 
 
-Lemma stp_extend : forall v1 G1 T1 T2,
-                       stp G1 T1 T2 ->
-                       stp (v1::G1) T1 T2.
-Proof. intros. induction H; eauto. Qed.
 
 
-Lemma valtp_extend : forall vs v v1 T,
-                       val_type vs v T ->
-                       val_type (v1::vs) v T.
-Proof. intros. induction H; eauto. Qed.
 
 Lemma index_extend : forall X vs n a (T: X),
                        index n vs = Some T ->
@@ -348,6 +363,25 @@ Proof.
   assert (beq_nat n (length vs) = false) as E. eapply beq_nat_false_iff; eauto.
   unfold index. unfold index in H. rewrite H. rewrite E. reflexivity.
 Qed.
+
+Lemma stp_extend : forall v1 G1 T1 T2,
+                       stp G1 T1 T2 ->
+                       stp (v1::G1) T1 T2.
+Proof. intros. induction H; eauto.
+       eapply stp_sel1. eapply index_extend; eauto.
+Qed.
+
+Lemma stp2_extend2 : forall v1 G1 G2 T1 T2,
+                       stp2 G1 T1 G2 T2 ->
+                       stp2 G1 T1 (v1::G2) T2.
+Proof. admit. Qed.
+
+
+Lemma valtp_extend : forall vs v v1 T,
+                       val_type vs v T ->
+                       val_type (v1::vs) v T.
+Proof. intros. induction H; eauto; econstructor; eauto; eapply stp2_extend2; eauto.  Qed.
+
 
 
 Lemma index_safe_ex: forall H1 G1 TF i,
@@ -383,12 +417,14 @@ Hint Constructors res_type.
 Hint Resolve not_stuck.
 
 
-Inductive stp2: venv -> ty -> venv -> ty -> Prop :=
-| stp2_refl: forall G1 G2 T,
-   stp2 G1 T G2 T.
-
-
 Hint Constructors stp2.
+
+
+Lemma stp2_trans: forall G1 G2 G3 T1 T2 T3,
+  stp2 G1 T1 G2 T2 ->
+  stp2 G2 T2 G3 T3 ->
+  stp2 G1 T1 G3 T3.
+Proof. admit. Qed.
 
 Lemma stp_to_stp2: forall G H T1 T2,
   wf_env H G ->
@@ -396,6 +432,13 @@ Lemma stp_to_stp2: forall G H T1 T2,
   stp2 H T1 H T2.
 Proof.
   intros. inversion H1. eauto.
+  (* sel *)
+  assert (exists v : vl, index x H = Some v /\ val_type H v (TMem T2)) as A.
+    eapply index_safe_ex. eauto. eauto.
+  destruct A as [? [? VT]].
+  inversion VT; try solve by inversion.  subst.
+    
+  eapply stp2_sel1; eauto. inversion H8. subst. eauto.
 Qed.
 
 Lemma valtp_widen: forall vf H1 H2 T1 T2,
@@ -403,7 +446,7 @@ Lemma valtp_widen: forall vf H1 H2 T1 T2,
   stp2 H1 T1 H2 T2 ->
   val_type H2 vf T2.
 Proof.
-  intros. inversion H; inversion H0; subst T2; subst; eauto.
+  intros. inversion H; econstructor; eauto; eapply stp2_trans; eauto.
 Qed.
 
 
@@ -416,19 +459,19 @@ Lemma invert_abs: forall venv vf vx T1 T2,
     stp2 venv T1 (vx::vf::env) T3 /\
     stp2 (vx::vf::env) T4 venv T2.
 Proof.
-  intros. inversion H. repeat eexists; repeat eauto.
+  intros. inversion H; try solve by inversion. inversion H2. subst. repeat eexists; repeat eauto.
 Qed.
 
 Lemma invert_tabs: forall venv vf T1 T2,
   val_type venv vf (TAll T1 T2) ->
   exists env tenv y T3 T4,
-    vf = (vtabs env y) /\ 
+    vf = (vtabs env T3 y) /\ 
     wf_env env tenv /\
     has_type ((TMem T3)::tenv) y (open (TSel (length tenv)) T4) /\
-    stp2 venv T1 (vty::env) T3 /\
-    stp2 (vty::env) (open (TSel (length tenv)) T4) venv (open T1 T2).
+    stp2 venv T1 ((vty env T3)::env) T3 /\
+    stp2 ((vty env T3)::env) (open (TSel (length tenv)) T4) venv (open T1 T2).
 Proof.
-  intros. inversion H. repeat eexists; repeat eauto. eapply H5. eapply se_refl.
+  intros. inversion H; try solve by inversion. inversion H2. subst. repeat eexists; repeat eauto. eapply H1. eapply se_refl.
   (* final stp2 *)admit.
   (* from val_type we get wf: (open T1 T2) <: (open T1 T2) *)
 Qed.
@@ -446,8 +489,8 @@ Proof.
   (* 0 *)   intros. inversion H.
   (* S n *) intros. destruct e; inversion H; inversion H0.
   
-  Case "True".  eapply not_stuck. eapply v_bool.
-  Case "False". eapply not_stuck. eapply v_bool.
+  Case "True".  eapply not_stuck. eapply v_bool; eauto.
+  Case "False". eapply not_stuck. eapply v_bool; eauto.
 
   Case "Var".
     destruct (index_safe_ex venv0 tenv0 T i) as [v [I V]]; eauto. 
@@ -483,6 +526,7 @@ Proof.
     eapply not_stuck. eapply valtp_widen; eauto.
     
   Case "Abs". intros. inversion H. inversion H0.
+    subst. inversion H11. subst.
     eapply not_stuck. eapply v_abs; eauto.
 
   Case "TApp".
@@ -498,17 +542,18 @@ Proof.
         [env1 [tenv [y0 [T3 [T4 [EF [WF [HTY [STX STY]]]]]]]]]. eauto.
     (* now we know it's a closure, and we have has_type evidence *)
 
-    assert (res_type (vty::env1) res (open (TSel (length tenv)) T4)) as HRY.
+    assert (res_type ((vty env1 T3)::env1) res (open (TSel (length tenv)) T4)) as HRY.
       SCase "HRY".
         subst. eapply IHn. eauto. eauto.
         (* wf_env x *) econstructor. eapply v_ty. 
         (* wf_env   *) eauto.
-
+    eauto. eauto.
     inversion HRY as [? vy].
 
     eapply not_stuck. eapply valtp_widen; eauto.
 
   Case "TAbs". intros. inversion H. inversion H0.
+    subst. inversion H11. subst.
     eapply not_stuck. eapply v_tabs; eauto.
     
 Qed.
